src/program_proof/simple/simple.v
@@ -10,25 +10,39 @@ From Perennial.program_proof Require Import txn.txn_proof buftxn.buftxn_proof ma
 From Perennial.program_proof Require Import proof_prelude.
 From Perennial.program_proof Require Import disk_lib.
 From Perennial.Helpers Require Import NamedProps Map List range_set.
+From Perennial.algebra Require Import log_heap.
 From Perennial.program_logic Require Import spec_assert.
 From Perennial.goose_lang.lib Require Import slice.typed_slice into_val.
+From Perennial.program_proof Require Import simple.spec.
 
-Module simple.
-  Definition ino := list u8.
-  Definition t := gmap nat ino.
-End simple.
+(* XXX lift somewhere higher up *)
+Canonical Structure u64O := leibnizO u64.
+Canonical Structure u8O := leibnizO u8.
+Canonical Structure asyncO T := leibnizO (async T).
 
 Section heap.
 Context `{!crashG Σ}.
 Context `{!buftxnG Σ}.
-Context `{!invG Σ}.
+Context `{!inG Σ (ghostR $ gmapO u64O $ asyncO $ list u8)}.
 Implicit Types (stk:stuckness) (E: coPset).
 
 Record simple_names := {
   simple_txn : @txn_names Σ;
-  simple_src : gen_heapG nat simple.ino Σ;
+  simple_state : gname;
+  simple_src : gen_heapG u64 (async (list u8)) Σ;
   simple_lockmapghs : list (gen_heapG u64 bool Σ);
 }.
+
+Variable P : SimpleNFS.State -> iProp Σ.
+Context `{!forall σ, Timeless (P σ)}.
+
+Definition is_source γ : iProp Σ :=
+  ∃ (src: SimpleNFS.State),
+    own γ.(simple_state) (● Excl' src) ∗
+    (* If we were doing a refinement proof, the top-level source_state would
+     * own the ◯ of this ghost variable.. *)
+    gen_heap_ctx (hG := γ.(simple_src)) src ∗
+    P src.
 
 Definition LogSz : nat := 513.
 Definition InodeSz : nat := 128.
@@ -37,13 +51,13 @@ Definition NumInodes : nat := 4096 / InodeSz.
 Definition encodes_inode (len: u64) (blk: u64) data : Prop :=
   has_encoding data (EncUInt64 len :: EncUInt64 blk :: nil).
 
-Definition inum2addr inum := Build_addr LogSz (inum * InodeSz * 8).
+Definition inum2addr (inum : u64) := Build_addr LogSz (int.nat inum * InodeSz * 8).
 Definition blk2addr blk := Build_addr blk 0.
 
-Definition is_inode_enc γ (inum: nat) (len: u64) (blk: u64) : iProp Σ :=
+Definition is_inode_enc γ (inum: u64) (len: u64) (blk: u64) : iProp Σ :=
   ∃ (ibuf : defs.inode_buf),
-    ⌜ encodes_inode len blk (vec_to_list ibuf) ⌝ ∗
-    mapsto_txn γ.(simple_txn) (inum2addr inum) (existT _ (defs.bufInode ibuf)).
+    "%Hinode_encodes" ∷ ⌜ encodes_inode len blk (vec_to_list ibuf) ⌝ ∗
+    "Hinode_enc_mapsto" ∷ mapsto_txn γ.(simple_txn) (inum2addr inum) (existT _ (defs.bufInode ibuf)).
 
 Definition is_inode_data γ (len : u64) (blk: u64) (contents: list u8) : iProp Σ :=
   ∃ (bbuf : Block),
@@ -51,18 +65,18 @@ Definition is_inode_data γ (len : u64) (blk: u64) (contents: list u8) : iProp �
     "%Hdisklen" ∷ ⌜ len = length contents ⌝ ∗
     "Hdiskblk" ∷ mapsto_txn γ.(simple_txn) (blk2addr blk) (existT _ (defs.bufBlock bbuf)).
 
-Definition is_inode_disk γ (inum: nat) (state: simple.ino) : iProp Σ :=
+Definition is_inode_disk γ (inum: u64) (state: list u8) : iProp Σ :=
   ∃ (blk: u64),
-    is_inode_enc γ inum (length state) blk ∗
-    is_inode_data γ (length state) blk state.
+    "Hinode_enc" ∷ is_inode_enc γ inum (length state) blk ∗
+    "Hinode_data" ∷ is_inode_data γ (length state) blk state.
 
-Definition is_inode_mem (l: loc) (inum: nat) (len: u64) (blk: u64) : iProp Σ :=
+Definition is_inode_mem (l: loc) (inum: u64) (len: u64) (blk: u64) : iProp Σ :=
   "Hinum" ∷ l ↦[Inode.S :: "Inum"] #inum ∗
   "Hisize" ∷ l ↦[Inode.S :: "Size"] #len ∗
   "Hidata" ∷ l ↦[Inode.S :: "Data"] #blk.
 
-Theorem wp_inum2Addr inum :
-  {{{ ⌜ inum < NumInodes ⌝ }}}
+Theorem wp_inum2Addr (inum : u64) :
+  {{{ ⌜ int.nat inum < NumInodes ⌝ }}}
     inum2Addr #inum
   {{{ RET (addr2val (inum2addr inum)); True }}}.
 Proof.
@@ -72,6 +86,7 @@ Proof.
   rewrite /addr2val /inum2addr /=.
   rewrite /LogSz /InodeSz.
   replace (word.add (word.divu (word.sub 4096 8) 8) 2)%Z with (U64 513) by reflexivity.
+(*
   replace (word.mul (word.mul inum 128) 8)%Z with (U64 (inum * 128 * 8)%nat).
   { iApply "HΦ". done. }
 
@@ -81,6 +96,7 @@ Proof.
   intros.
   word_cleanup.
   admit.
+*)
 Admitted.
 
 Theorem wp_block2addr bn :
@@ -94,12 +110,16 @@ Proof.
   iApply "HΦ". done.
 Qed.
 
-Theorem wp_ReadInode γ inum len blk (btxn : loc) bufm :
+Definition covered_inodes : gset u64 :=
+  rangeSet 2 (NumInodes-2).
+
+Theorem wp_ReadInode γ (inum : u64) len blk (btxn : loc) bufm :
   {{{ is_buftxn btxn bufm γ.(simple_txn) ∗
       is_inode_enc γ inum len blk ∗
-      ⌜ inum < NumInodes ⌝ }}}
+      ⌜ inum ∈ covered_inodes ⌝ }}}
     ReadInode #btxn #inum
   {{{ l, RET #l;
+      is_buftxn btxn bufm γ.(simple_txn) ∗
       is_inode_enc γ inum len blk ∗
       is_inode_mem l inum len blk }}}.
 Proof.
@@ -107,8 +127,10 @@ Proof.
 
   wp_call.
   wp_apply (wp_inum2Addr); auto.
+(*
   replace (#(LitInt (word.mul 128 8))) with (#1024%nat) by reflexivity.
   wp_apply (wp_BufTxn__ReadBuf with "[$Hbuftxn]").
+*)
 
   (* Need the [is_inode_enc] to be actually lifted into the buftxn active transaction.
    * Need to solve two problems to get there:
@@ -117,27 +139,20 @@ Proof.
    *)
 Admitted.
 
-Definition is_source γ : iProp Σ :=
-  ∃ (src: simple.t),
-    (* Really we want to say [source_ctx ∗ source_state src] here,
-     * but we have not yet defined the [language] for our simple NFS server.. *)
-    gen_heap_ctx (hG := γ.(simple_src)) src.
+Definition is_inode_stable γ (inum: u64) : iProp Σ :=
+  ∃ (state: list u8),
+    "Hinode_state" ∷ mapsto (hG := γ.(simple_src)) inum 1%Qp (sync state) ∗
+    "Hinode_disk" ∷ is_inode_disk γ inum state.
 
-Definition is_inode_stable γ (inum64: u64) : iProp Σ :=
-  ∃ (inum: nat) (state: simple.ino),
-    ⌜ inum64 = inum ⌝ ∗
-    mapsto (hG := γ.(simple_src)) inum 1%Qp state ∗
-    is_inode_disk γ inum state.
-
-Definition covered_inodes : gset u64 :=
-  rangeSet 2 (NumInodes-2).
+Definition N := nroot .@ "simplenfs".
 
 Definition is_fs γ (nfs: loc) : iProp Σ :=
   ∃ (txn lm : loc),
-    readonly (nfs ↦[Nfs.S :: "t"] #txn) ∗
-    readonly (nfs ↦[Nfs.S :: "l"] #lm) ∗
-    is_txn txn γ.(simple_txn) ∗
-    is_lockMap lm γ.(simple_lockmapghs) covered_inodes (is_inode_stable γ).
+    "#Hfs_txn" ∷ readonly (nfs ↦[Nfs.S :: "t"] #txn) ∗
+    "#Hfs_lm" ∷ readonly (nfs ↦[Nfs.S :: "l"] #lm) ∗
+    "#Histxn" ∷ is_txn txn γ.(simple_txn) ∗
+    "#Hislm" ∷ is_lockMap lm γ.(simple_lockmapghs) covered_inodes (is_inode_stable γ) ∗
+    "#Hsrc" ∷ inv N (is_source γ).
 
 Theorem wp_Inode__Read γ ip inum len blk (btxn : loc) (offset : u64) (bytesToRead : u64) bufm contents :
   {{{ is_buftxn btxn bufm γ.(simple_txn) ∗
@@ -268,6 +283,186 @@ Proof.
     { admit. }
 
   - admit.
+Admitted.
+
+Definition is_fh (s : Slice.t) (fh : u64) : iProp Σ :=
+  ∃ vs,
+    "#Hfh_slice" ∷ readonly (is_slice_small s u8T 1 vs) ∗
+    "%Hfh_enc" ∷ ⌜ has_encoding vs (EncUInt64 fh :: nil) ⌝.
+
+Opaque slice_val.
+
+Theorem wp_fh2ino s i :
+  {{{ is_fh s i }}}
+    fh2ino (slice_val s, #())%V
+  {{{ RET #i; True }}}.
+Proof.
+  iIntros (Φ) "Hfh HΦ".
+  iNamed "Hfh".
+  iMod (readonly_load with "Hfh_slice") as (q) "Hslice"; first by solve_ndisj.
+  wp_call.
+  wp_call.
+  wp_apply (wp_new_dec with "Hslice"); first by eauto.
+  iIntros (dec) "Hdec".
+  wp_apply (wp_Dec__GetInt with "Hdec").
+  iIntros "Hdec".
+  wp_pures.
+  iApply "HΦ".
+  done.
+Qed.
+
+Theorem wp_validInum (i : u64) :
+  {{{ True }}}
+    validInum #i
+  {{{ (valid : bool), RET #valid; ⌜ valid = true -> i ∈ covered_inodes ⌝ }}}.
+Proof.
+  iIntros (Φ) "_ HΦ".
+  wp_call.
+  wp_if_destruct.
+  { iApply "HΦ". done. }
+  wp_if_destruct.
+  { iApply "HΦ". done. }
+  wp_call.
+  wp_if_destruct.
+  { iApply "HΦ". done. }
+  iApply "HΦ".
+  iPureIntro. intuition.
+  rewrite /covered_inodes /NumInodes /InodeSz.
+  replace (4096 `div` 128) with (32) by reflexivity.
+  replace (word.divu (U64 4096) (U64 128)) with (U64 32) in Heqb1 by reflexivity.
+  apply rangeSet_lookup; try lia.
+  split.
+  { admit. }
+  { word. }
+Admitted.
+
+Opaque nfstypes.READ3res.S.
+
+Theorem wp_NFSPROC3_READ γ (nfs : loc) (fh : u64) (fhslice : Slice.t) (offset : u64) (count : u32) (Q : SimpleNFS.res (bool * SimpleNFS.buf) -> iProp Σ) :
+  {{{ is_fs γ nfs ∗
+      is_fh fhslice fh ∗
+      ∀ σ σ' r E,
+        ⌜relation.denote (SimpleNFS.wrapper fh (SimpleNFS.read fh offset count)) σ σ' r⌝ -∗
+        ( P σ ={E}=∗ P σ' ∗ Q r )
+  }}}
+    Nfs__NFSPROC3_READ #nfs (slice_val fhslice, #(), (#offset, (#count, #())))%V
+(*
+      (struct.mk nfstypes.READ3args.S [
+        "File" ::= struct.mk nfstypes.Nfs_fh3.S [
+          "Data" ::= slice_val fhslice
+        ];
+        "Offset" ::= #offset;
+        "Count" ::= #count
+      ])
+*)
+  {{{ (ok : bool) v,
+      RET v;
+      if ok then
+        ⌜ getField_f nfstypes.READ3res.S "Status" v = #0 ⌝ ∗
+        ∃ (eof : bool) (dataslice : Slice.t) r,
+          Q r
+      else
+        ⌜ getField_f nfstypes.READ3res.S "Status" v ≠ #0 ⌝
+  }}}.
+Proof.
+  iIntros (Φ) "(Hfs & #Hfh & Hfupd) HΦ".
+  iNamed "Hfs".
+
+  wp_call.
+  wp_apply wp_ref_of_zero; first by auto.
+  iIntros (reply) "Hreply".
+  wp_apply util_proof.wp_DPrintf.
+  wp_loadField.
+  wp_apply (wp_buftxn_Begin with "Histxn").
+  iIntros (buftx) "Hbuftxn".
+  wp_apply (wp_fh2ino with "Hfh").
+  wp_pures.
+  wp_apply (wp_validInum).
+  iIntros (valid) "%Hvalid".
+  wp_if_destruct.
+  { wp_pures.
+    wp_apply (wp_storeField_struct with "Hreply"); first by auto.
+    iIntros "Hreply".
+
+    wp_load.
+    iApply ("HΦ" $! false).
+    iPureIntro.
+    Transparent nfstypes.READ3res.S.
+    simpl.
+    Opaque nfstypes.READ3res.S.
+    congruence.
+  }
+
+  wp_loadField.
+  wp_apply (wp_LockMap__Acquire with "[$Hislm]"); first by auto.
+  iIntros "[Hstable Hlocked]".
+  iNamed "Hstable".
+  iNamed "Hinode_disk".
+  wp_apply (wp_ReadInode with "[$Hbuftxn $Hinode_enc]"); first by auto.
+  iIntros (ip) "(Hbuftxn & Hinode_enc & Hinode_mem)".
+  wp_apply (wp_Inode__Read with "[$Hbuftxn $Hinode_mem $Hinode_data]").
+  iIntros (resSlice eof vs) "(HresSlice & Hbuftxn & Hinode_mem & Hinode_data & %Hvs & %Heof)".
+  wp_apply (wp_BufTxn__CommitWait with "[$Hbuftxn Hfupd Hinode_state]").
+  {
+    iModIntro.
+    iExists _.
+    iSplitR.
+    { admit. }
+    iIntros "Hown".
+    iInv "Hsrc" as ">Hopen" "Hclose".
+    iDestruct "Hopen" as (src) "(Hsrcown & Hsrcheap & HP)".
+    iDestruct (gen_heap_valid with "Hsrcheap Hinode_state") as "%Hsrc_fh".
+    iDestruct ("Hfupd" with "[] HP") as "Hfupd".
+    {
+      iPureIntro.
+      simpl.
+      monad_simpl.
+      simpl.
+      rewrite Hsrc_fh.
+      simpl.
+      econstructor. { econstructor. auto. }
+      instantiate (3 := true).
+      simpl.
+      monad_simpl.
+    }
+    iMod "Hfupd" as "[HP HQ]".
+    iMod ("Hclose" with "[Hsrcown Hsrcheap HP]").
+    { iModIntro. iExists _. iFrame. }
+    iModIntro.
+
+    (* XXX this might be simpler using Tej's buftxn spec *)
+    admit.
+  }
+
+  iIntros (ok) "Hok".
+  wp_if_destruct.
+  2: {
+    wp_apply (wp_storeField_struct with "Hreply"); first by auto.
+    iIntros "Hreply".
+
+    wp_loadField.
+    (* XXX commitWait stole my [Hinode_state]! *)
+(*
+    wp_apply (wp_LockMap__Release with "[$Hislm $Hlocked Hinode_enc Hinode_data Hinode_state]").
+    { iExists _. iFrame.
+      iExists _. iFrame. }
+
+    wp_load.
+    iApply ("HΦ" $! false).
+    iPureIntro.
+    Transparent nfstypes.READ3res.S.
+    simpl.
+    Opaque nfstypes.READ3res.S.
+    congruence.
+*)
+    admit.
+  }
+
+  iDestruct (struct_fields_split with "Hreply") as "Hreply".
+  iNamed "Hreply".
+  wp_storeField.
+  (* XXX how to do anything with [struct.fieldRef]? *)
+  admit.
 Admitted.
 
 End heap.
